CopyPropagation.v
@@ -1,0 +1,323 @@
+Require Import CSet Le.
+
+Require Import Plus Util AllInRel Map.
+Require Import Val Var Env EnvTy IL ParamsMatch Sim Alpha Coherence Fresh.
+
+Require Import Liveness.
+
+Set Implicit Arguments.
+Unset Printing Records.
+
+Fixpoint subst (ϱ:env var) (s:stmt) : stmt :=
+  match s with
+    | stmtExp x e s => let x' := fresh (lookup_set ϱ (freeVars s)) in
+                       stmtExp x' (rename_exp ϱ e) (subst (ϱ[x <- x']) s)
+    | stmtIf x s t => stmtIf (ϱ x) (subst ϱ s) (subst ϱ t)
+    | stmtGoto l Y => stmtGoto l (lookup_list ϱ Y)
+    | stmtReturn x => stmtReturn (ϱ x)
+    | stmtLet Z s t => let Z' := fresh_list (lookup_set ϱ (freeVars s)) (length Z) in
+                       stmtLet Z' (subst (ϱ[Z <-- Z']) s) (subst ϱ t)
+  end.  
+
+Fixpoint copyPropagate (ϱ:var -> var) (s:stmt) : stmt :=
+  match s with
+   | stmtExp x (Var y) s => copyPropagate (ϱ[x <- ϱ y]) s
+   | stmtExp x e s => let x' := fresh (lookup_set ϱ (freeVars s)) in
+                        stmtExp x' e (copyPropagate (ϱ[x <- x']) s)
+   | stmtIf x s1 s2 => stmtIf (ϱ x) (copyPropagate ϱ s1) (copyPropagate ϱ s2)
+   | stmtGoto l Y => stmtGoto l (lookup_list ϱ Y)
+   | stmtReturn x => stmtReturn (ϱ x)
+   | stmtLet Z s1 s2 => 
+     let Z' := fresh_list (lookup_set ϱ (freeVars s1)) (length Z) in
+     stmtLet Z' (copyPropagate (ϱ[Z <-- Z']) s1) (copyPropagate ϱ s2)
+   end.
+
+Notation "f '[' L ']'" := (lookup_list f L) (at level 70).
+
+Instance ctxeq_equivalence : Equivalence ctxeq.
+Proof.
+  hnf; intros. constructor.
+  hnf; intros. eapply ctxeq_simeq; reflexivity.
+  hnf; intros. eapply ctxeq_simeq; eapply ctxeq_simeq in H; symmetry; eauto.
+  hnf; intros. eapply ctxeq_simeq. eapply ctxeq_simeq in H; eapply ctxeq_simeq in H0;
+                                   transitivity y; eauto.
+Qed.
+
+Lemma comp_update (ϱ1: var -> var) x (v:val) (E:var -> val) D
+ : x ∈ D ->
+   injective_on D ϱ1
+   -> agree_on D ((ϱ1 ∘ E) [x <- v]) ((ϱ1 ∘ E[ϱ1 x <- v])).
+Proof.
+  intros. unfold comp.  hnf; intros. lud.
+  rewrite e in H4. exfalso. eapply H4. reflexivity.
+  exfalso. eapply H3. eapply H0; eauto. 
+Qed.
+
+Lemma comp_update_2 (ϱ1: var -> var) x (v:var) (E:var -> val) D
+ : agree_on D ((ϱ1 ∘ E) [x <- E v]) ((ϱ1[x <- v] ∘ E)).
+Proof.
+  intros. unfold comp.  hnf; intros. lud.
+Qed.
+
+Lemma comp_update_3 (ϱ1: var -> var) x (v:val) (E:var -> val) D
+ : ϱ1 x = x 
+   -> x ∉ lookup_set ϱ1 (D\{{x}})
+   -> agree_on D ((ϱ1 ∘ E) [x <- v]) ((ϱ1 ∘ E[x <- v])).
+Proof.
+  intros. unfold comp.  hnf; intros. lud. 
+  rewrite <- H in e. exfalso. eapply H5. rewrite H2. eauto.
+  exfalso. eapply H0. eapply lookup_set_spec. intuition. 
+  eexists; split; eauto. cset_tac; eauto.
+Qed.
+
+Lemma exp_rename_shift E e ϱ
+ : exp_eval (ϱ ∘ E) e = exp_eval E (rename_exp ϱ e).
+Proof.
+  general induction e; simpl; eauto.
+  - rewrite IHe1, IHe2; reflexivity.
+Qed.
+
+Lemma rename_contr s ϱ ϱ'
+: rename ϱ (rename ϱ' s) = rename (ϱ' ∘ ϱ) s.
+Proof.
+  unfold comp.
+  general induction s; simpl;  f_equal; eauto. eapply rename_exp_comp.
+  rewrite <- comp_lookup_list. reflexivity.
+  rewrite <- comp_lookup_list. reflexivity.
+Qed.
+
+Lemma exp_subst_agree (ϱ ϱ':var->var) (E E' : var -> val) (e:exp)
+: agree_on (Exp.freeVars e) (ϱ ∘ E) (ϱ' ∘ E')
+  -> exp_eval E (rename_exp ϱ e) = exp_eval E' (rename_exp ϱ' e).
+Proof.
+  general induction e; simpl; eauto. f_equal; eapply H. simpl; cset_tac; eauto.
+  - simpl in *. erewrite IHe1, IHe2; try reflexivity; eapply agree_on_incl; eauto;
+                cset_tac; intuition.
+Qed.
+
+
+Lemma agree_on_comp_fresh (ϱ:var -> var) (E: var -> var) x x' y (D: set var)
+  : x' ∉ lookup_set ϱ D 
+    -> agree_on D (ϱ [x <- y] ∘ E)
+                (ϱ [x <- x'] ∘ E [x' <- E y]).
+Proof.
+  intros. hnf; intros. unfold comp.
+  lud. exfalso; eauto.
+  exfalso. eapply H. eapply lookup_set_spec. intuition. eexists x0; intuition.
+Qed.
+
+Lemma agree_on_comp_fresh_both (ϱ ϱ':var -> var) (E E': var -> var) x y y' (v:val) (D: set var)
+ : y ∉ lookup_set ϱ D
+   -> y' ∉ lookup_set ϱ' D
+   -> agree_on (D\{{x}}) (ϱ ∘ E) (ϱ' ∘ E')
+   -> agree_on D (ϱ [x <- y] ∘ E [y <- v]) (ϱ' [x <- y'] ∘ E' [y' <- v]).
+Proof.
+  intros. hnf; intros. simpl. unfold comp.
+  lud. hnf in H4; congruence.
+  exfalso. eapply H. eapply lookup_set_spec; intuition. eexists x0; intuition.
+  exfalso. hnf in H4; congruence.
+  exfalso. hnf in H4; congruence.
+  exfalso. eapply H0. eapply lookup_set_spec; intuition. eexists x0; intuition.
+  eapply H1; eauto. cset_tac; intuition.
+Qed.
+
+Lemma agree_on_comp_fresh_both_list (ϱ ϱ':var -> var) (E E': var -> var) Z Y Y' (VL: list val) (D: set var)
+ : length Z = length Y
+   -> length Y = length Y'
+   -> length Y' = length VL
+   -> unique Y
+   -> unique Y'
+   -> (of_list Y) ∩ lookup_set ϱ D [=] ∅
+   -> (of_list Y') ∩ lookup_set ϱ' D [=] ∅
+   -> agree_on (D\of_list Z) (ϱ ∘ E) (ϱ' ∘ E')
+   -> agree_on D (ϱ [Z <-- Y] ∘ E [Y <-- VL]) (ϱ' [Z <-- Y'] ∘ E' [Y' <-- VL]).
+Proof.
+  intros.
+  eapply length_length_eq in H.
+  eapply length_length_eq in H0.
+  eapply length_length_eq in H1.
+  hnf; intros. simpl. unfold comp. destruct_prop (x ∈ of_list Z).
+  clear H6.
+  general induction H; inv H0; inv H1; simpl in * |- *.
+  exfalso. eapply (not_in_empty x); eauto.
+  hnf; intros. unfold comp. lud.
+  exfalso. eapply H9; reflexivity.
+  exfalso. 
+  destruct_prop (x0 ∈ of_list XL).
+  assert (y ∈ of_list YL). rewrite e.
+  eapply update_with_list_lookup_in; eauto using length_eq_length.
+  eapply H2. eapply InA_in in H12. eauto.
+  assert (ϱ x0 = y).
+  eapply update_with_list_lookup_not_in; eauto. 
+  refine (not_in_empty y _). rewrite <- H4. cset_tac; intuition.
+  exfalso. eapply H8; reflexivity.
+  exfalso. eapply H8; reflexivity.
+  exfalso. 
+  destruct_prop (x0 ∈ of_list XL).
+  assert (y0 ∈ of_list YL0). rewrite e.
+  eapply update_with_list_lookup_in; eauto using length_eq_length,length_eq_trans.
+  eapply H3. eapply InA_in in H12. eauto.
+  assert (ϱ' x0 = y0).
+  eapply update_with_list_lookup_not_in; eauto. 
+  refine (not_in_empty y0 _). rewrite <- H5. cset_tac; intuition.
+  eapply (IHlength_eq _ _ _ _ _ _ D); eauto. intuition. intuition.
+  cset_tac; intuition. eapply H4; split; eauto. cset_tac; intuition.
+  cset_tac; intuition. eapply H5; split; eauto. cset_tac; intuition.
+  cset_tac; intuition.
+  assert ((ϱ [Z <-- Y]) x = ϱ x). 
+  erewrite (update_with_list_lookup_not_in ϱ); eauto.
+  assert ((ϱ' [Z <-- Y']) x = ϱ' x). 
+  erewrite (update_with_list_lookup_not_in ϱ'); eauto.
+  rewrite H8, H9.
+  assert ((E [Y <-- VL]) (ϱ x) = E (ϱ x)). 
+  erewrite (update_with_list_lookup_not_in E); eauto.
+  cset_tac; intuition. eapply H4; split; eauto. 
+  eapply lookup_set_spec. intuition. eexists; eauto.
+  assert ((E' [Y' <-- VL]) (ϱ' x) = E' (ϱ' x)). 
+  erewrite (update_with_list_lookup_not_in E'); eauto.
+  cset_tac; intuition. eapply H5; split; eauto. 
+  eapply lookup_set_spec. intuition. eexists; eauto.
+  rewrite H10, H11. eapply H6. cset_tac; intuition.
+Qed.
+
+
+Lemma subst_fresh L L' (E E':var -> val) s (ϱ ϱ':var->var)
+ : simL L L'
+   -> agree_on (freeVars s) (ϱ ∘ E) (ϱ' ∘ E')
+   -> sim (L, E, subst ϱ s)
+          (L', E' , subst ϱ' s).
+Proof.
+  general induction s; simpl in * |- *.
+  case_eq (exp_eval E (rename_exp ϱ e)); intros.
+  eapply simS; try eapply plusO.
+  constructor; eauto.
+  econstructor. erewrite <- exp_subst_agree; eauto. 
+  eapply agree_on_incl; eauto. cset_tac; intuition.
+  eapply IHs; eauto. 
+  eapply agree_on_comp_fresh_both; eauto using fresh_spec.
+  eapply agree_on_incl; eauto. cset_tac; intuition.
+  eapply simE; try eapply star_refl; simpl; eauto. stuck. stuck.
+  erewrite exp_subst_agree in def; eauto. rewrite def in H1. congruence.
+  eapply agree_on_incl. eapply agree_on_sym. eauto. cset_tac; intuition.
+  + case_eq (val2bool (E (ϱ x))); intros.
+    eapply simS; try eapply plusO.
+    econstructor; eauto.
+    econstructor; eauto. specialize (H0 x). unfold comp in H0.
+    rewrite <- H0; eauto. cset_tac; intuition.
+    eapply IHs1; eauto. eapply agree_on_incl; eauto. cset_tac; intuition.
+    eapply simS; try eapply plusO.
+    econstructor 3; eauto.
+    econstructor 3; eauto. specialize (H0 x). unfold comp in H0.
+    rewrite <- H0; eauto. cset_tac; intuition.
+    eapply IHs2; eauto. eapply agree_on_incl; eauto. cset_tac; intuition.
+  + destruct (get_dec L (counted l)). destruct s as [[]].
+    destruct_prop (length block_Z = length Y). 
+    unfold simL in H.
+    edestruct AIR4_length; try eassumption; dcr.
+    edestruct get_length_eq; try eassumption.
+    edestruct AIR4_nth as [?[?]]; try eassumption; dcr. 
+    simpl in *. repeat get_functional; subst.
+    inv H9. eapply simS; try eapply plusO.
+    econstructor; eauto. simpl. rewrite lookup_list_length. congruence.
+    econstructor; eauto. simpl. rewrite lookup_list_length. congruence.
+    simpl. unfold updE. 
+    assert (lookup_list E (lookup_list ϱ Y) = lookup_list E' (lookup_list ϱ' Y)).
+    repeat rewrite <- comp_lookup_list.
+    eauto using lookup_list_agree.
+    rewrite H2. eapply H14. repeat rewrite lookup_list_length. congruence. congruence.
+    eapply simE; try eapply star_refl; eauto; stuck.
+    get_functional; subst. eapply n. simpl in *. rewrite len.
+    rewrite lookup_list_length; eauto.
+    edestruct AIR4_length; try eassumption; dcr.
+    edestruct get_length_eq; try eassumption.
+    edestruct AIR4_nth as [?[?]]; try eassumption; dcr. 
+    simpl in *. repeat get_functional; subst.
+    inv H9; simpl in *. eapply n. rewrite lookup_list_length in len. congruence.
+    eapply simE; try eapply star_refl; eauto; stuck; eauto.
+    edestruct AIR4_length; try eassumption; dcr.
+    edestruct get_length_eq; try eassumption. eauto.
+  + eapply simE; try eapply star_refl; simpl; eauto; try stuck. 
+    f_equal. eapply H0; simpl; cset_tac; eauto.
+  + simpl in * |- *.
+    eapply simS; try eapply plusO.
+    econstructor. econstructor.
+    eapply IHs2; eauto. eapply simL_extension; eauto. 
+    hnf; intros. eapply IHs1; eauto. 
+    eapply agree_on_comp_fresh_both_list;
+      repeat rewrite fresh_list_length; eauto;
+      eauto using fresh_list_unique, fresh_list_spec.
+    repeat rewrite fresh_list_length in *. congruence. 
+    repeat rewrite fresh_list_length in *. 
+    
+    eapply agree_on_incl; eauto. cset_tac; intuition.
+    rewrite fresh_list_length; eauto.
+    rewrite fresh_list_length; eauto. 
+    eapply agree_on_incl; eauto. cset_tac; intuition.
+Qed.
+
+Lemma sim_CP s ϱ 
+: simeq (copyPropagate ϱ s) (subst ϱ s).
+Proof. 
+  general induction s; simpl in * |- *. 
+  + destruct e; hnf; intros.
+    - one_step. reflexivity. reflexivity. 
+      unfold simeq in IHs. eapply IHs; eauto.
+    - eapply sim_expansion_closed.
+      Focus 2. eapply star_refl.
+      Focus 2. eapply S_star. econstructor. simpl. reflexivity. eapply star_refl.
+      simpl in * |- *.
+      refine (sim_trans (IHs _ _ _) _ ); eauto.
+      eapply subst_fresh. eapply simL_refl. eapply agree_on_comp_fresh.
+      eapply fresh_spec.
+    - 
+      exfalso; clear_all; admit.
+  + transitivity (stmtIf (ϱ x) (copyPropagate ϱ s1) (subst ϱ s2)). 
+    eapply (simeq_contextual (ctxIfT (ϱ x) _ ctxHole)); eauto.
+    eapply (simeq_contextual (ctxIfS (ϱ x) ctxHole _)); eauto.
+  + eapply simeq_refl.
+  + eapply simeq_refl.
+  + eapply simeq_trans.
+    eapply (simeq_contextual (ctxLetT _ _ ctxHole)); eauto.
+    eapply (simeq_contextual (ctxLetS _ ctxHole _)). eapply IHs1; eauto.
+Qed.
+
+Lemma lookup_set_id {X} `{H : OrderedType X} (s : set X)
+: s [=] lookup_set id s.
+Proof.
+  unfold lookup_set. 
+  hnf; intros. rewrite map_spec; unfold id; simpl; intuition.
+  eexists a; intuition. destruct H0; cset_tac.
+Qed.
+
+Instance fresh_morph
+: Proper (Equal ==> eq) fresh.
+Proof.
+  unfold Proper, respectful; intros.
+  admit.
+Qed.
+
+Lemma subst_id s
+  : simeq s (subst id s).
+Proof.
+  general induction s; simpl;
+  repeat rewrite <- lookup_set_id.
+  
+Admitted.
+
+Lemma CP_tv s s' C C' D D'
+  : ssa C s C' -> ssa D s' D'
+  -> copyPropagate id s = copyPropagate id s'
+  -> simeq s s'.
+Proof.
+  intros. 
+  pose proof (simeq_trans (subst_id _) (simeq_sym (sim_CP s _ ))); eauto.
+  pose proof (simeq_trans (subst_id _) (simeq_sym (sim_CP s' _ ))); eauto.
+  eapply simeq_sym in H3. rewrite <- H1 in H3.
+  eapply simeq_trans; eauto.  
+Qed.
+
+(* 
+*** Local Variables: ***
+*** coq-load-path: (("." "Lvc")) ***
+*** End: ***
+*)
